\documentclass{assignment}

\usepackage{amsmath}
\begin{document}

\assignmentTitle{Mykola Vaskevych}{22372199}{assets/images.jpg}
{Foundations of Computer Science 2}{Homework 8}

\section*{Task 1}
Use the while rule to prove that the following program segment is correct:
\[\{ n\geq 1 \wedge i = 1 \wedge sum = 0 \wedge f = 1\}\]
\[while \quad (i \leq n) \quad \{\]
\[sum = sum + f;\]
\[i = i + 1;\]
\[f = f * 1;\}\]

\section*{Defining the Invariant}
\begin{center}
    \begin{tabular}{|c|c|c|c|}
        sum & i & f \\
        \hline
         0 & 1 & 1 \\
         1 & 2 & 2 \\
         3 & 3 & 6 \\
         9 & 4 & 24 \\
         33 & 5 & 120\\
         \hline
    \end{tabular}
\end{center}
So, out invariant will be: \[\{sum = \sum_{j=1}^{j=i-1} j! \wedge f = i! \wedge i \leq n + 1 \}\]
Then we can write out Hoare Triple:
\[\{D \wedge I\} C \{I\}\]

\[\{i \leq n \wedge sum = \sum_{j=1}^{j=i-1} j! \wedge f = i! \wedge i \leq n + 1 \}\quad sum = sum + f; \quad i = i + 1; \quad f = f * i \quad \{\sum_{j=1}^{j=i-1}j! \wedge f = i! \wedge i \leq n + 1 \} \]
\newpage
\section*{Concatenation Rule}
\begin{enumerate}
    \item  
        \[\{i \leq n \wedge sum = \sum_{j=1}^{j=i-1} j! \wedge f = i! \wedge i \leq n + 1\}\quad sum = sum + f \{R_1\} \]
    \item
        \[\{R_1\} \quad i = i + 1 \quad \{R_2\}\]
    \item
        \[\{R_2\} \quad f = f * i \quad \{sum = \sum_{j=1}^{j=i-1}j! \wedge f = i! \wedge i \leq n + 1\}\]

\end{enumerate}

\section*{Assignment Rule for (3)}
    \[R_2 = Q_{E_1}^V\]
    \[Q_{E_1}^V: \{sum = \sum_{j=1}^{j=i-1}j! \wedge f = i! \wedge i \leq n + 1\}_{f=f*i}^f\]
    \[Q_{E_1}^V: \{sum = \sum_{j=1}^{j=i-1}j! \wedge f*i = i! \wedge i \leq n + 1\}\]
    \[Q_{E_1}^V: \{sum = \sum_{j=1}^{j=i-1}j! \wedge f = (i-1)! \wedge i \leq n + 1\}\]
\section*{Assignment Rule for (2)}
    \[R_1 = Q_{E_2}^V\]
    \[Q_{E_2}^V: \{sum = \sum_{j=1}^{j=i-1}j! \wedge f = (i-1)! \wedge i \leq n + 1\}_{i = i + 1}^{i}\]
    \[Q_{E_2}^V: \{sum = \sum_{j=1}^{j=i+1-1}j! \wedge f = (i + 1 -1)! \wedge i+1 \leq n +1\}\]
    \[Q_{E_2}^V: \{sum = \sum_{j=1}^{j=i}j! \wedge f = i! \wedge i+1 \leq n +1\}\]
\section*{Assignment Rule for (1)}
    \[Q_{E_3}^V: \{sum = \sum_{j=1}^{j=i}j! \wedge f = i! \wedge i+1 \leq n +1\}_{sum+f}^{sum}\]
    \[Q_{E_3}^V: \{sum + f = \sum_{j=1}^{j=i}j! \wedge f = i! \wedge i+1 \leq n +1\}\] 

\section*{Finally}
\[P: \{i \leq n \wedge sum = \sum_{j=1}^{j=i-1} j! \wedge f = i! \wedge i \leq n + 1\}\]
\[in P: \{i \leq n\} \Rightarrow \{i \leq n+1\}\]
\[P: \{i \leq n \wedge sum = \sum_{j=1}^{j=i-1} j! \wedge f = i! \}\]
\[Q_{E_3}^V: \{sum + f = \sum_{j=1}^{j=i}j! \wedge f = i! \wedge i+1 \leq n +1\}\]
\[Q_{E_3}^V: \{sum = \sum_{j=1}^{j=i} j! - f \wedge f = i! \wedge i+1 \leq n +1\}\]
\[Q_{E_3}^V: \{sum = \sum_{j=1}^{j=i} j! - i! \wedge f = i! \wedge i+1 \leq n +1\}\]
\[Q_{E_3}^V: \{sum = \sum_{j=1}^{j=i-1} j! \wedge f = i! \wedge i+1 \leq n +1\}\]

\[\{i \leq n \wedge sum = \sum_{j=1}^{j=i-1} j! \wedge f = i! \} \Rightarrow \{sum = \sum_{j=1}^{j=i-1} j! \wedge f = i! \wedge i+1 \leq n +1\} \]
\begin{enumerate}
    \item
        \[\{i \leq n \Rightarrow i + 1 \leq n+1\}\]
    \item
        \[\{f = i! \Rightarrow f = 1!\}\]
    \item 
        \[\{sum = \sum_{j=1}^{j=i-1} j!\} \Rightarrow \{sum = \sum_{j=1}^{j=i-1} j!\}\]
\end{enumerate}
\[P \Rightarrow Q_{E_3}^V\]
So, we proved that this segment of code is correct.
\end{document}


